Splinter/SplinterTreeInvariants.i.dfy
@@ -18,11 +18,11 @@ module SplinterTreeInvariantMod {
   import opened SplinterTreeMachineMod
   import Nat_Order
 
-  // TODO; Might need to change this to table about both IM and IMStable
-  lemma StableFraming(v: Variables, cache0: CacheIfc.Variables, cache1: CacheIfc.Variables, sb:Superblock)
-    requires DiskViewsEquivalentForSeq(cache0.dv, cache1.dv, IReadsSeq(v, cache0))
-    ensures IMStable(cache0, sb) == IMStable(cache1, sb)
-  {
-  }
+//  // TODO; Might need to change this to table about both IM and IMStable
+//  lemma StableFraming(v: Variables, cache0: CacheIfc.Variables, cache1: CacheIfc.Variables, sb:Superblock)
+//    requires DiskViewsEquivalentForSeq(cache0.dv, cache1.dv, IReadsSeq(v, cache0))
+//    ensures IM(cache0, sb) == IM(cache1, sb)
+//  {
+//  }
 
 }
